various things

src/dafny/Probability/Probability.dfy
@@ -1,67 +1,121 @@
 module RNG {
   type rng = nat -> bool
 
-  function hd(s: rng): bool {
+  // Definition 14
+  function shd(s: rng): bool {
     s(0)
   }
 
-  function tl(s: rng): rng {
+  // Definition 14
+  function stl(s: rng): rng {
     (n: nat) => s(n+1)
   }
 
-  function cons(a: bool, s: rng, n: nat): bool {
+  // Definition 14
+  function scons(a: bool, s: rng, n: nat): bool {
     if n == 0 then 
       a 
     else 
       s(n-1)
   }
 
-  function take(n: nat, s: rng): seq<bool> {
+  // Definition 14
+  function stake(n: nat, s: rng): seq<bool> {
     if n == 0 then
       []
     else
-      [hd(s)] + take(n-1, tl(s))
+      [shd(s)] + stake(n-1, stl(s))
   }
 
-  function drop(n: nat, s: rng): rng {
+  // Definition 14
+  function sdrop(n: nat, s: rng): rng {
     if n == 0 then
       s
     else
-      drop(n-1, tl(s))
+      sdrop(n-1, stl(s))
   }
 
-  function dest(s: rng): (bool, rng) {
-    (hd(s), tl(s))
+  // Definition 14
+  function sdest(s: rng): (bool, rng) {
+    (shd(s), stl(s))
   }
 
+  // Definition 15
+  ghost function siter<A>(h: A -> bool, t: A -> A, x: A): rng {
+    assume false;
+    (n: nat) => scons(h(x), siter(h, t, t(x)), n)
+  }
+
+  // Definition 16
+  ghost function mirror(s: rng): rng {
+    (n: nat) => scons(!shd(s), stl(s), n)
+  }
+
+  // Definition 17
   ghost function prefix_set(l: seq<bool>): iset<rng> {
-    iset s: rng | take(|l|, s) == l
+    iset s: rng | stake(|l|, s) == l
   }
 
+  // Definition 17
   ghost function prefix_seq(l: seq<bool>, a: bool): seq<bool> {
     if l == [] then
       [a]
     else
       [l[0]] + prefix_seq(l[1..], a)
   }
-  
+
+  // Equation (2.45)
+  lemma LemmaHdCons(h: bool, t: rng) 
+    ensures shd((n: nat) => scons(h, t, n)) == h
+  {}
+
+  // Equation (2.46)
+  lemma LemmaTlCons(h: bool, t: rng, n: nat)
+    ensures stl((n: nat) => scons(h, t, n))(n) == t(n)
+  {}
+
+  // Equation (2.47), (2.48)
+  lemma LemmaHdtlDecomp(s: rng, n: nat) returns (x: (bool, rng))
+    ensures s(n) == scons(x.0, x.1, n)
+  {
+    x := (shd(s), stl(s));
+  }
+
+  // Equation (2.50)
+  lemma LemmaMirrorIdempotent(s: rng, n: nat) 
+    ensures mirror(mirror(s))(n) == s(n)
+  {}
+
+  // Equation (2.51)
+  lemma LemmaTlMirror(s: rng, n: nat)
+    ensures stl(mirror(s))(n) == stl(s)(n)
+  {}
 }
 
 module HurdMonad {
   import opened RNG
 
+  // Definition 29
   type Hurd<A> = rng -> (A, rng)
 
+  // Definition 29
   function Unit<A>(a: A): Hurd<A> {
     (s: rng) => (a, s)
   }
 
+  // Definition 29
   function Bind<A,B>(f: Hurd<A>, g: A -> Hurd<B>): Hurd<B> {
     (s: rng) =>
       var (a, s') := f(s);
       g(a)(s')
   }
 
+  function Map<A,B>(F: A -> B, f: Hurd<A>): Hurd<B> {
+    (s: rng) => 
+      var (a, s') := f(s);
+      (F(a), s')
+  }
+  
   function Join<A>(ff: Hurd<Hurd<A>>): Hurd<A> {
     (s: rng) =>
       var (f, s') := ff(s);
@@ -71,6 +125,30 @@ module HurdMonad {
   function Composition<A,B,C>(f: A -> Hurd<B>, g: B -> Hurd<C>): A -> Hurd<C> {
     (a: A) => Bind(f(a), g)
   }
+
+  // Monad law
+  lemma LemmaUnitalityJoin<A>(f: Hurd<A>, s: rng)
+    ensures Join(Map(Unit, f))(s) == Join(Unit(f))(s)
+  {
+    var (a, s') := f(s);
+    calc {
+      Join(Unit(f))(s);
+    ==
+      f(s);
+    ==
+      (a, s');
+    ==
+      Unit(a)(s');
+    ==
+      Join(Map(Unit, f))(s);
+    }
+  }
+  
+  // Monad law
+  // lemma LemmaAssociativityJoin<A>(fff: Hurd<Hurd<Hurd<A>>>)
+  //   ensures Join(Map(Join, fff)) == Join(Join(fff))
+  // {
+  // }
 }
 
 module Probability {
@@ -78,6 +156,7 @@ module Probability {
     iset x: T | false
   }
 
+  // Definition 4
   ghost predicate IsAlgebra<T(!new)>(event_space: iset<iset<T>>, sample_space: iset<T>) {
     && (forall e | e in event_space :: e <= sample_space)
     && EmptyIset() in event_space
@@ -102,6 +181,7 @@ module Probability {
     f(i) + CountableSum(f, i+1)
   }
 
+  // Definition 4
   ghost predicate IsSigmaAlgebra<T(!new)>(event_space: iset<iset<T>>, sample_space: iset<T>) {
     && IsAlgebra(event_space, sample_space)
     && forall f: nat -> iset<T> | (forall n :: f(n) in event_space) :: CountableUnion(f) in event_space 
@@ -111,28 +191,35 @@ module Probability {
 
   type MeasurableSpace<!T(!new)> = pair: MeasurableSpaceStructure | IsSigmaAlgebra(pair.event_space, pair.sample_space) witness *
 
+  // Definition 5
   ghost predicate IsPositive<T(!new)>(ms: MeasurableSpace<T>, mu: iset<T> -> real) {
     && mu(EmptyIset()) == 0.0
     && forall e | e in ms.event_space :: 0.0 <= mu(e)
   }
 
+  // Definition 5
   ghost predicate IsIncreasing<T(!new)>(ms: MeasurableSpace<T>, mu: iset<T> -> real) {
     forall e1, e2 | e1 in ms.event_space && e2 in ms.event_space && e1 <= e2 :: mu(e1) <= mu(e2)
   }
 
+  // Definition 5
+  ghost predicate IsAdditive<T(!new)>(ms: MeasurableSpace<T>, mu: iset<T> -> real) {
+    forall e1, e2 | e1 in ms.event_space && e2 in ms.event_space && e1 * e2 == EmptyIset() :: mu(e1) + mu(e2) == mu(e1 + e2)
+  }
+
+  // Definition 5
   ghost predicate IsCountablyAdditive<T(!new)>(ms: MeasurableSpace<T>, mu: iset<T> -> real) {
     forall f: nat -> iset<T> | (forall n :: f(n) in ms.event_space) && (forall m, n | m != n :: f(m) * f(n) == EmptyIset()) && (CountableUnion(f) in ms.event_space) :: (CountableSum((n: nat) => mu(f(n))) == mu(CountableUnion(f)))
   }
 
-  lemma {:axiom} LemmaIsBinaryAdditive<T(!new)>(ms: MeasurableSpace<T>, mu: iset<T> -> real, e1: iset<T>, e2: iset<T>)
+  // Equation (2.18)
+  lemma {:axiom} LemmaPosCountAddImpliesAdd<T(!new)>(ms: MeasurableSpace<T>, mu: iset<T> -> real)
+    requires IsPositive(ms, mu)
     requires IsCountablyAdditive(ms, mu)
-    requires e1 in ms.event_space
-    requires e2 in ms.event_space
-    requires e1 * e2 == EmptyIset()
-    ensures mu(e1) + mu(e2) == mu(e1 + e2)
+    ensures IsAdditive(ms, mu)
   
+  // Definition 6
   datatype MeasureSpaceStructure<!T(!new)> = Pair(ms: MeasurableSpace, mu: iset<T> -> real) 
-
   type MeasureSpace<!T(!new)> = pair: MeasureSpaceStructure | IsPositive(pair.ms, pair.mu) && IsCountablyAdditive(pair.ms, pair.mu) witness *
 
   ghost function PreImageOf<S(!new),T>(f: S -> T, domain: iset<S>, b: iset<T>): (a: iset<S>)
@@ -142,17 +229,31 @@ module Probability {
     iset x | x in domain && f(x) in b
   }
 
-  ghost predicate IsMeasurableFunction<S(!new),T(!new)>(ms1: MeasurableSpace<S>, ms2: MeasurableSpace<T>, f: S -> T)
-  {
+  // Definition 9
+  ghost predicate IsMeasurableFunction<S(!new),T(!new)>(ms1: MeasurableSpace<S>, ms2: MeasurableSpace<T>, f: S -> T) {
     forall e | e in ms2.event_space :: PreImageOf(f, ms1.sample_space, e) in ms1.event_space
   }
 
+  // Definition 12
   type ProbabilitySpace<!T(!new)> = ms: MeasureSpace | ms.mu(ms.ms.sample_space) == 1.0 witness *
+
+  // Definition 13
+  ghost predicate Independent<T(!new)>(ms: MeasureSpace<T>, e1: iset<T>, e2: iset<T>) {
+    && e1 in ms.ms.event_space
+    && e2 in ms.ms.event_space
+    && ms.mu(e1 * e2) == ms.mu(e1) * ms.mu(e2)
+  }
+
+  // Definition 13 
+  ghost predicate IndependentFamilies<T(!new)>(ms: MeasureSpace<T>, a: iset<iset<T>>, b: iset<iset<T>>) {
+    forall e1, e2 | e1 in a && e2 in b :: Independent(ms, e1, e2)
+  }
 }
 
 module RNGProbability {
   import opened RNG
   import opened Probability
+  import opened HurdMonad
 
   /* Axiomatisation for now */
   ghost const sample_space: iset<rng> := iset s: rng | true
@@ -168,11 +269,80 @@ module RNGProbability {
   // Equation (2.82)
   lemma {:axiom} RandomBit(n: nat)
     ensures 
-      var e := (iset s: rng | hd(drop(n, s)) == true);
+      var e := (iset s: rng | shd(sdrop(n, s)) == true);
       e in event_space && mu(e) == 0.5
+
+  // Definition 30
+  ghost predicate IsCompositional<A(!new)>(q: (() -> Hurd<A>) -> bool) {
+    && (forall a :: q(() => Unit(a)))
+    && (forall f: () -> Hurd<A>, g: A -> Hurd<A> :: q(f) && forall a :: q(() => g(a)) ==> q(() => Bind(f(), g)))
+  }
+
+  // function Dice(): Hurd<nat> 
+
+  // function TwoDice(): Hurd<nat> {
+  //   Bind(Dice(), (x: nat) => Bind(Dice(), (y: nat) => Unit(x + y)))
+  // }
+
+  // Definition 37
+  function ProbWhileCut<A>(c: A -> bool, b: A -> Hurd<A>, n: nat, a: A): Hurd<A> {
+    if n == 0 then
+      Unit(a)
+    else 
+      if c(a) then 
+        Bind(b(a), a' => ProbWhileCut(c, b, n-1, a')) 
+      else 
+        Unit(a)
+  }
+
+  // // Equation (3.25)
+  // ghost function ProbWhile<A>(c: A -> bool, b: A -> Hurd<A>, a: A, s: rng, arb: (A, rng)): (A, rng) {
+  //   var xs: iset<nat> := iset n | !(c(ProbWhileCut(c, b, n, a)(s).0));
+  //   if xs != {} then
+  //     var n: nat :| n in xs && (forall m | m in xs :: n <= m);
+  //     ProbWhileCut(c, b, n, a)(s)
+  //   else
+  //     arb
+  // }
+
+
+  // Definition 44
+  function ProbUntil<A>(b: Hurd<A>, c: A -> bool): Hurd<A> 
+
+  // Definition 47
+  function ProbBinomial(n: nat): Hurd<nat> {
+    if n == 0 then
+      Unit(0)
+    else 
+      var f: nat -> Hurd<nat> := 
+        (m: nat) =>
+          var g: bool -> Hurd<nat> := (b: bool) => Unit(if b then m + 1 else m);
+          Bind(sdest, g);
+      Bind(ProbBinomial(n - 1), f)
+  }
+
+  // Definition 48
+  function ProbUnif(n: nat): Hurd<nat> {
+    if n == 0 then
+      Unit(0)
+    else
+      var f: nat -> Hurd<nat> := 
+        (m: nat) => 
+          var g: bool -> Hurd<nat> := (b: bool) => Unit(if b then 2 * m + 1 else 2 * m);
+          Bind(sdest, g);
+      Bind(ProbUnif(n / 2), f)
+  }
+
+  // Definition 49
+  function ProbUniform(n: nat): Hurd<nat> 
+    requires n > 0
+  {
+    ProbUntil(ProbUnif(n-1), (x: nat) => x < n)
+  }
+
 }
 
-module Examples {
+module ExampleFlip {
   import opened RNG
   import opened HurdMonad
   import opened RNGProbability
@@ -180,13 +350,14 @@ module Examples {
 
   datatype Coin = Head | Tail
 
+  // p15
   ghost function RNGSatisfyingSpec<A,B>(spec: (A, B) -> bool, f: A -> Hurd<B>, a: A): iset<rng> {
     iset s: rng | spec(a, f(a)(s).0)
   }
 
-  function Flip(x: ()): Hurd<Coin> 
+  function Flip(): Hurd<Coin> 
   {
-    (s: rng) => (if s(0) then Head else Tail, tl(s))
+    (s: rng) => (if s(0) then Head else Tail, stl(s))
   }
 
   function Spec1(a: (), b: Coin): bool {
@@ -198,27 +369,22 @@ module Examples {
   }
 
   lemma AboutFlip() 
-    requires RNGSatisfyingSpec(Spec1, Flip, ()) in event_space
-    requires RNGSatisfyingSpec(Spec2, Flip, ()) in event_space
-    ensures mu(RNGSatisfyingSpec(Spec1, Flip, ())) == 0.5 
-    ensures mu(RNGSatisfyingSpec(Spec2, Flip, ())) == 0.5 
+    requires RNGSatisfyingSpec(Spec1, (x: ()) => Flip(), ()) in event_space
+    requires RNGSatisfyingSpec(Spec2, (x: ()) => Flip(), ()) in event_space
+    ensures mu(RNGSatisfyingSpec(Spec1, (x: ()) => Flip(), ())) == 0.5 
+    ensures mu(RNGSatisfyingSpec(Spec2, (x: ()) => Flip(), ())) == 0.5 
   {
-    var e1 := RNGSatisfyingSpec(Spec1, Flip, ());
-    var e2 := RNGSatisfyingSpec(Spec2, Flip, ());
-    assert e1 == iset s: rng | s(0) == true;
-    assert e2 == iset s: rng | s(0) == false;
+    var e1 := RNGSatisfyingSpec(Spec1, (x: ()) => Flip(), ());
+    var e2 := RNGSatisfyingSpec(Spec2, (x: ()) => Flip(), ());
     RandomBit(0);
-    assert mu((iset s: rng | hd(drop(0, s)) == true)) == 0.5;
-    assert mu(e1) == 0.5 by { assert e1 == (iset s: rng | hd(drop(0, s)) == true); }
+    assert mu((iset s: rng | shd(sdrop(0, s)) == true)) == 0.5;
+    assert mu(e1) == 0.5 by { assert e1 == (iset s: rng | shd(sdrop(0, s)) == true); }
     assert e1 + e2 == sample_space;
-    assert e1 * e2 == EmptyIset();
     assert IsSigmaAlgebra(event_space, sample_space) by { LemmaProbabilitySpace(); }
-    assert sample_space in event_space by { LemmaSampleSpaceInAlgebra(event_space, sample_space); }
-    assert e1 + e2 in event_space;
     var ms := MeasurableSpaceStructure.Pair(event_space, sample_space);
+    assert IsPositive(ms, mu) by { LemmaProbabilitySpace(); }
     assert IsCountablyAdditive(ms, mu) by { LemmaProbabilitySpace(); }
-    LemmaIsBinaryAdditive(ms, mu, e1, e2);
-    assert mu(e1 + e2) == mu(e1) + mu(e2);
+    LemmaPosCountAddImpliesAdd(ms, mu);
     assert mu(sample_space) == 1.0 by { LemmaProbabilitySpace(); }
     assert mu(e2) == 0.5;
   }
